src/Language/PIR.v
@@ -12,3 +12,22 @@ Definition PIRLang : Language :=
   ; const := fun i => Constant (Some' (ValueOf DefaultUniInteger i))
   |}
 .
+
+
+From PlutusCert Require Import RelationalModel.
+
+Require Import Lists.List.
+Import ListNotations.
+
+Lemma LR_forward t t' ty :
+  LR_logically_approximate [] [] t t' ty ->
+  forward PIRLang PIRLang t t'.
+Proof.
+  intros H_LR.
+  destruct H_LR as [H_ty_t H_ty_t' .
+
+bigstep L (app L p (const L n)) (const L r).
+
+
+eval (Apply t Constant (Some' (ValueOf DefaultUniInteger i))) v i ->
+eval (Apply t ())
